coq: ZF: Class.Relation.HasValueAt

coq/ZF/Class/Relation/Eval.v
@@ -4,46 +4,17 @@ Require Import ZF.Class.Relation.Domain.
 Require Import ZF.Class.Empty.
 Require Import ZF.Class.Relation.Functional.
 Require Import ZF.Class.Relation.FunctionalAt.
-Require Export ZF.Class.Relation.IsValueAt.
+Require Export ZF.Class.Relation.HasValueAt.
 Require Import ZF.Class.Inter2.
 Require Import ZF.Class.Small.
 Require Import ZF.Set.Core.
 Require Import ZF.Set.OrdPair.
 
-(* Predicate expressing the fact that the class F has a value at a.             *)
-Definition HasValueAt (F:Class) (a:U) : Prop := exists y, IsValueAt F a y.
-
-(* The class HasValueAt F is an intersection.                                   *)
-Proposition HasValueAtAsInter : forall (F:Class),
-  HasValueAt F :~: FunctionalAt F :/\: domain F.
-Proof.
-  intros F a. split; intros H1.
-  - destruct H1 as [y [H1 H2]]. split. 1: assumption.
-    exists y. assumption.
-  - destruct H1 as [H1 H2]. destruct H2 as [y H2]. exists y.
-    apply IsValueAt.WhenFunctionalAt; assumption.
-Qed.
-
-Proposition HasValueAtWhenFunctionalAt : forall (F:Class) (a:U),
-  FunctionalAt F a -> HasValueAt F a <-> domain F a.
-Proof.
-  intros F a H1. split; intros H2.
-  - apply HasValueAtAsInter in H2. apply H2.
-  - apply HasValueAtAsInter. split; assumption.
-Qed.
-
-(* When F is functional, the classes HasValueAt F and domain F coincide.        *)
-Proposition HasValueAtWhenFunctional : forall (F:Class),
-  Functional F -> HasValueAt F :~: domain F.
-Proof.
-  intros F H1 a.
-  apply HasValueAtWhenFunctionalAt, IsFunctionalAt. assumption.
-Qed.
-
 (* Evaluate the class F at a.                                                   *)
 Definition eval (F:Class) (a:U) : Class := fun x =>
   exists y, x :< y /\ IsValueAt F a y.
 
+(* Evaluation is compatible with class equivalence.                             *)
 Proposition EquivCompat : forall (F G:Class) (a:U),
   F :~: G -> eval F a :~: eval G a.
 Proof.
@@ -80,7 +51,7 @@ Proposition WhenFunctionalAt : forall (F:Class) (a y:U),
   FunctionalAt F a -> domain F a -> F :(a,y): <-> eval F a :~: toClass y.
 Proof.
   intros F a y H1 H2.
-  apply WhenHasValueAt, HasValueAtWhenFunctionalAt; assumption.
+  apply WhenHasValueAt, HasValueAt.WhenFunctionalAt; assumption.
 Qed.
 
 (* If F is functional and a lies in domain of F then F (a,y) iff eval F a = y.  *)
@@ -88,7 +59,7 @@ Proposition WhenFunctional : forall (F:Class) (a y:U),
   Functional F -> domain F a -> F :(a,y): <-> eval F a :~: toClass y.
 Proof.
   intros F a y H1 H2.
-  apply WhenHasValueAt, HasValueAtWhenFunctional; assumption.
+  apply WhenHasValueAt, HasValueAt.WhenFunctional; assumption.
 Qed.
 
 (* If F has no value at a then eval F a is the empty class.                     *)
@@ -106,7 +77,7 @@ Proposition WhenNotFunctionalAt : forall (F:Class) (a:U),
   ~ FunctionalAt F a -> eval F a :~: :0:.
 Proof.
   intros F a H1. apply WhenNotHasValueAt. intros H2. apply H1.
-  apply HasValueAtAsInter. assumption.
+  apply HasValueAt.AsInter. assumption.
 Qed.
 
 (* If a is not in domain of F then eval F a is the empty class.                 *)
@@ -114,7 +85,7 @@ Proposition WhenNotInDomain : forall (F:Class) (a:U),
   ~ domain F a -> eval F a :~: :0:.
 Proof.
   intros F a H1. apply WhenNotHasValueAt. intros H2. apply H1.
-  apply HasValueAtAsInter. assumption.
+  apply HasValueAt.AsInter. assumption.
 Qed.
 
 (* The value of F at a is a always a small class.                               *)
